@prefix : <http://www.semanticweb.org/anon/ontologies/2025/4/Blocks/> .
@prefix owl: <http://www.w3.org/2002/07/owl#> .
@prefix rdf: <http://www.w3.org/1999/02/22-rdf-syntax-ns#> .
@prefix xml: <http://www.w3.org/XML/1998/namespace> .
@prefix xsd: <http://www.w3.org/2001/XMLSchema#> .
@prefix rdfs: <http://www.w3.org/2000/01/rdf-schema#> .
@base <http://www.semanticweb.org/anon/ontologies/2025/4/Blocks/> .

<http://www.semanticweb.org/anon/ontologies/2025/4/Blocks> rdf:type owl:Ontology .

#################################################################
#    Object Properties
#################################################################

###  http://www.semanticweb.org/anon/ontologies/2025/4/Blocks#on
:on rdf:type owl:ObjectProperty ;
    rdfs:domain :Block ;
    rdfs:comment "Describes the location of a block (either another block or a table). A block does not have a location while it is being held." .


###  http://www.semanticweb.org/anon/ontologies/2025/4/Blocks#onBlock
:onBlock rdf:type owl:ObjectProperty ;
         rdfs:subPropertyOf :on ;
         rdf:type owl:FunctionalProperty ;
         rdfs:range :Block ,
                    :Blocked ;
         rdfs:comment "A relation between two blocks stacked on top of each other. A block can be on top of at most one other block." .


###  http://www.semanticweb.org/anon/ontologies/2025/4/Blocks#onTable
:onTable rdf:type owl:ObjectProperty ;
         rdfs:subPropertyOf :on ;
         rdfs:range :Table ;
         rdfs:comment "A relation between a block and the table it is currently on." .


#################################################################
#    Classes
#################################################################

###  http://www.semanticweb.org/anon/ontologies/2025/4/Blocks#Block
:Block rdf:type owl:Class ;
       rdfs:subClassOf [ rdf:type owl:Restriction ;
                         owl:onProperty :on ;
                         owl:someValuesFrom owl:Thing
                       ] ;
       owl:disjointWith :Table ;
       rdfs:comment "A block in the block's world. Every block must have a location (object property \"on\"). A block is not a table." .


###  http://www.semanticweb.org/anon/ontologies/2025/4/Blocks#Blocked
:Blocked rdf:type owl:Class ;
         rdfs:comment "A block is blocked if there is another block on it or it is currently being held." .


###  http://www.semanticweb.org/anon/ontologies/2025/4/Blocks#Holding
:Holding rdf:type owl:Class ;
         rdfs:subClassOf :Block ,
                         :Blocked ;
         rdfs:comment "Designates the block that is currently being held." .


###  http://www.semanticweb.org/anon/ontologies/2025/4/Blocks#Table
:Table rdf:type owl:Class ;
       rdfs:comment "The table in the block's world. The implicit assumption is that the is only one table, but this ontology does not enforce this." .


#################################################################
#    General axioms
#################################################################

[ rdf:type owl:Restriction ;
  owl:onProperty :onBlock ;
  owl:someValuesFrom owl:Thing ;
  owl:disjointWith [ rdf:type owl:Restriction ;
                     owl:onProperty :onTable ;
                     owl:someValuesFrom owl:Thing
                   ]
] .


###  Generated by the OWL API (version 4.5.29.2024-05-13T12:11:03Z) https://github.com/owlcs/owlapi
